start proving exec_implies_oldexec

bedrock2/src/bedrock2/Semantics.v
@@ -1,5 +1,5 @@
 Require Import coqutil.sanity coqutil.Byte.
-Require Import coqutil.Tactics.fwd.
+Require Import coqutil.Tactics.fwd coqutil.Tactics.Tactics.
 Require Import coqutil.Map.Properties.
 Require coqutil.Map.SortedListString.
 Require Import bedrock2.Syntax coqutil.Map.Interface coqutil.Map.OfListWord.
@@ -207,28 +207,9 @@ Module exec. Section WithParams.
           exists l', map.putmany_of_list_zip binds retvs l = Some l' /\
           post t' m' l') ->
       exec (cmd.call binds fname arges) t m l post
-  (* | interact: forall binds action arges args t m l post mKeep mGive mid, *)
-  (*     map.split m mKeep mGive -> *)
-  (*     eval_call_args l arges = Some args -> *)
-  (*     ext_spec t mGive action args mid -> *)
-  (*     (forall mReceive resvals, mid mReceive resvals -> *)
-  (*         exists l', map.putmany_of_list_zip binds resvals l = Some l' /\ *)
-  (*         forall m', map.split m' mKeep mReceive -> *)
-  (*         post (cons ((mGive, action, args), (mReceive, resvals)) t) m' l') -> *)
-  (*     exec (cmd.interact binds action arges) t m l post. *)
-           .
+  .
 
   Context {word_ok: word.ok word} {mem_ok: map.ok mem} {ext_spec_ok: ext_spec.ok ext_spec}.
-
-  (* Lemma interact_cps: forall binds action arges args t m l post mKeep mGive, *)
-  (*     map.split m mKeep mGive -> *)
-  (*     eval_call_args l arges = Some args -> *)
-  (*     ext_spec t mGive action args (fun mReceive resvals => *)
-  (*         exists l', map.putmany_of_list_zip binds resvals l = Some l' /\ *)
-  (*         forall m', map.split m' mKeep mReceive -> *)
-  (*         post (cons ((mGive, action, args), (mReceive, resvals)) t) m' l') -> *)
-  (*     exec (cmd.interact binds action arges) t m l post. *)
-  (* Proof. intros. eauto using interact. Qed. *)
 
   Lemma seq_cps: forall c1 c2 t m l post,
       exec c1 t m l (fun t' m' l' => exec c2 t' m' l' post) ->
@@ -266,41 +247,219 @@ Module exec. Section WithParams.
   End WithParams.
 End exec. Notation exec := exec.exec.
 
-Section WithParams.
+Module oldexec. Section WithParams.
   Context {width: Z} {BW: Bitwidth width} {word: word.word width} {mem: map.map word byte}.
   Context {locals: map.map String.string word}.
   Context {ext_spec: ExtSpec}.
+  Section WithEnv.
+  Context (e: env).
 
-  Implicit Types (l: locals) (m: list mem) (post: trace -> list mem -> list word -> Prop).
+  Implicit Types post : trace -> mem -> locals -> Prop. (* COQBUG: unification finds Type instead of Prop and fails to downgrade *)
+  Inductive exec: cmd -> trace -> mem -> locals ->
+                  (trace -> mem -> locals -> Prop) -> Prop :=
+  | skip: forall t m l post,
+      post t m l ->
+      exec cmd.skip t m l post
+  | set: forall x e t m l post v,
+      eval_expr l e = Some v ->
+      post t m (map.put l x v) ->
+      exec (cmd.set x e) t m l post
+  | unset: forall x t m l post,
+      post t m (map.remove l x) ->
+      exec (cmd.unset x) t m l post
+  | load: forall x sz e t m l post a v,
+      eval_expr l e = Some a ->
+      load sz m a = Some v ->
+      post t m (map.put l x v) ->
+      exec (cmd.load x sz e) t m l post
+  | store: forall sz ea ev t m l post a v m',
+      eval_expr l ea = Some a ->
+      eval_expr l ev = Some v ->
+      store sz m a v = Some m' ->
+      post t m' l ->
+      exec (cmd.store sz ea ev) t m l post
+  | stackalloc: forall x n body t mSmall l post,
+      Z.modulo n (bytes_per_word width) = 0 ->
+      (forall a mStack mCombined,
+        anybytes a n mStack ->
+        map.split mCombined mSmall mStack ->
+        exec body t mCombined (map.put l x a)
+          (fun t' mCombined' l' =>
+            exists mSmall' mStack',
+              anybytes a n mStack' /\
+              map.split mCombined' mSmall' mStack' /\
+              post t' mSmall' l')) ->
+      exec (cmd.stackalloc x n body) t mSmall l post
+  | if_true: forall t m l e c1 c2 post v,
+      eval_expr l e = Some v ->
+      word.unsigned v <> 0 ->
+      exec c1 t m l post ->
+      exec (cmd.cond e c1 c2) t m l post
+  | if_false: forall e c1 c2 t m l post v,
+      eval_expr l e = Some v ->
+      word.unsigned v = 0 ->
+      exec c2 t m l post ->
+      exec (cmd.cond e c1 c2) t m l post
+  | seq: forall c1 c2 t m l post mid,
+      exec c1 t m l mid ->
+      (forall t' m' l', mid t' m' l' -> exec c2 t' m' l' post) ->
+      exec (cmd.seq c1 c2) t m l post
+  | while_false: forall e c t m l post v,
+      eval_expr l e = Some v ->
+      word.unsigned v = 0 ->
+      post t m l ->
+      exec (cmd.while e c) t m l post
+  | while_true: forall e c t m l post v mid,
+      eval_expr l e = Some v ->
+      word.unsigned v <> 0 ->
+      exec c t m l mid ->
+      (forall t' m' l', mid t' m' l' -> exec (cmd.while e c) t' m' l' post) ->
+      exec (cmd.while e c) t m l post
+  | call: forall binds fname arges t m l post params rets fbody args lf mid,
+      map.get e fname = Some (params, rets, fbody) ->
+      eval_call_args l arges = Some args ->
+      map.of_list_zip params args = Some lf ->
+      exec fbody t m lf mid ->
+      (forall t' m' st1, mid t' m' st1 ->
+          exists retvs, map.getmany_of_list st1 rets = Some retvs /\
+          exists l', map.putmany_of_list_zip binds retvs l = Some l' /\
+          post t' m' l') ->
+      exec (cmd.call binds fname arges) t m l post
+  .
 
-  Definition call e fname t m args post :=
-    exists argnames retnames body,
-      map.get e fname = Some (argnames, retnames, body) /\
-      exists l, map.of_list_zip argnames args = Some l /\
-        exec e body t m l (fun t' m' l' => exists rets,
-          map.getmany_of_list l' retnames = Some rets /\ post t' m' rets).
+  Context {word_ok: word.ok word} {mem_ok: map.ok mem} {ext_spec_ok: ext_spec.ok ext_spec}.
 
-  Lemma weaken_call: forall e fname t m args post1,
-      call e fname t m args post1 ->
-      forall post2, (forall t' m' rets, post1 t' m' rets -> post2 t' m' rets) ->
-      call e fname t m args post2.
+  Lemma seq_cps: forall c1 c2 t m l post,
+      exec c1 t m l (fun t' m' l' => exec c2 t' m' l' post) ->
+      exec (cmd.seq c1 c2) t m l post.
+  Proof. intros. eauto using seq. Qed.
+
+  Lemma weaken: forall t l m s post1,
+      exec s t m l post1 ->
+      forall post2,
+        (forall t' m' l', post1 t' m' l' -> post2 t' m' l') ->
+        exec s t m l post2.
   Proof.
-    unfold call. intros. fwd.
-    do 4 eexists. 1: eassumption.
-    do 2 eexists. 1: eassumption.
-    eapply exec.weaken. 1: eassumption.
-    cbv beta. clear -H0. intros. fwd. eauto.
+    induction 1; intros; try solve [econstructor; eauto].
+    - eapply stackalloc. 1: assumption.
+      intros.
+      eapply H1; eauto.
+      intros. fwd. eauto 10.
+    - eapply call.
+      4: eapply IHexec.
+      all: eauto.
+      intros.
+      edestruct H3 as (? & ? & ? & ? & ?); [eassumption|].
+      eauto 10.
   Qed.
 
-  Lemma extend_env_call: forall e1 e2,
+  End WithEnv.
+
+  Lemma extend_env: forall e1 e2,
       map.extends e2 e1 ->
-      forall f t m rets post,
-      call e1 f t m rets post ->
-      call e2 f t m rets post.
+      forall c t m l post,
+      exec e1 c t m l post ->
+      exec e2 c t m l post.
+  Proof. induction 2; try solve [econstructor; eauto]. Qed.
+
+  End WithParams.
+End oldexec. Notation oldexec := oldexec.exec.
+
+Section WithParams.
+  Context {width: Z} {BW: Bitwidth width} {word: word.word width} {mem: map.map word byte}.
+  Context {locals: map.map String.string word}.
+  Context {word_ok: word.ok word} {mem_ok: map.ok mem}.
+  Context {ext_spec: ExtSpec}.
+
+  Implicit Types (l: locals) (m: list mem) (post: trace -> list mem -> locals -> Prop).
+  
+  Inductive all_disj : list mem -> Prop :=
+  | nil_disj : all_disj []
+  | cons_disj m mi : all_disj m ->
+                     map.disjoint mi (fold_right map.putmany map.empty m) ->
+                     all_disj (mi :: m).
+
+  Lemma all_disj_alt mi m :
+    all_disj (mi :: m) ->
+    forall mj, In mj m ->
+          map.disjoint mi mj.
+  Proof. Admitted.
+
+  Lemma all_disj_putmany_commute m :
+    all_disj m ->
+    fold_right map.putmany map.empty m = fold_right (fun x y => map.putmany y x) map.empty m.
   Proof.
-    unfold call. intros. fwd. repeat eexists.
-    - eapply H. eassumption.
-    - eassumption.
-    - eapply exec.extend_env; eassumption.
+    induction m; intros Hdisj; [reflexivity|]. inversion Hdisj. subst.
+    specialize (IHm ltac:(assumption)). simpl. rewrite <- IHm. apply map.putmany_comm.
+    assumption.
   Qed.
+
+  Lemma all_disj_get m mi a v :
+    all_disj m ->
+    In mi m ->
+    map.get mi a = Some v ->
+    map.get (fold_right map.putmany map.empty m) a = Some v.
+  Proof.
+    induction m.
+    - intros _ contra. destruct contra.
+    - intros Hdisj Hin Hget. inversion Hdisj. subst. specialize (IHm H1).
+      rewrite all_disj_putmany_commute by assumption. simpl.
+      rewrite <- all_disj_putmany_commute by assumption.
+      inversion Hin; subst.
+      + Search (map.get (map.putmany _ _)). apply map.get_putmany_right. assumption.
+      + rewrite map.get_putmany_left.
+        -- apply IHm; assumption.
+        -- pose proof all_disj_alt as H'. specialize (H' _ _ Hdisj _ H).
+           clear -H' Hget. cbv [map.disjoint] in H'. specialize (H' a).
+           destruct (map.get a0 a); [|reflexivity]. exfalso. eapply H'; eauto.
+  Qed.
+
+  Lemma all_disj_getmany_of_tuple sz m mi keys v :
+    all_disj m ->
+    In mi m ->
+    @map.getmany_of_tuple _ _ _ mi sz keys = Some v ->
+    @map.getmany_of_tuple _ _ _ (fold_right map.putmany map.empty m) sz keys  = Some v.
+  Proof.
+    intros Hdisj HIn. pose proof all_disj_get as Hget.
+    specialize Hget with (1 := Hdisj) (2 := HIn).
+    induction sz.
+    - destruct keys. cbv [map.getmany_of_tuple]. simpl. auto.
+    - destruct keys. cbn [map.getmany_of_tuple]. cbv [map.getmany_of_tuple]. simpl.
+      destruct_one_match; [|congruence]. apply Hget in E. rewrite E.
+      destruct_one_match; [|congruence]. intros H. inversion H. clear H. subst.
+      apply IHsz in E0. cbv [map.getmany_of_tuple] in E0. rewrite E0. reflexivity.
+  Qed.      
+
+  Lemma all_disj_load m sz mi a v :
+    all_disj m ->
+    In mi m ->
+    load sz mi a = Some v ->
+    load sz (fold_right map.putmany map.empty m) a = Some v.
+  Proof.
+    intros Hdisj Hin Hload. cbv [load load_Z load_bytes] in *.
+    pose proof all_disj_getmany_of_tuple as Hget.
+    specialize Hget with (1 := Hdisj) (2 := Hin).
+    destruct_one_match_hyp; [|congruence]. inversion Hload. subst. clear Hload.
+    destruct_one_match_hyp; [|congruence]. inversion E. subst. clear E.
+    apply Hget in E0. rewrite E0. reflexivity.
+  Qed.
+  
+  Lemma exec_implies_oldexec e s t m l post :
+    all_disj m ->
+    exec e s t m l post ->
+    oldexec e s t (fold_right map.putmany map.empty m) l
+      (fun t mflat' l =>
+         exists m', mflat' = fold_right map.putmany map.empty m' /\
+         post t m' l).
+  Proof.
+    intros H0 H. revert H0. induction H; intros Hdisj; try solve [econstructor; eauto].
+    - econstructor; eauto using all_disj_load.
+    - econstructor; eauto.
+
+      
+                
+    
+    
+    
+    
 End WithParams.
